\newpage
\section{Beispiele}
\mdfsetup{backgroundcolor=blue!08}
\begin{mdframed}
\begin{center}
    $A = \begin{pmatrix}
        a & b & c \\
        d & e & f \\
        g & h & i
    \end{pmatrix}$
    \quad $\det A = {\color{orange}a \cdot e \cdot i + b \cdot f \cdot g + c \cdot d \cdot h}\text{ }{\color{blue} -g \cdot e \cdot c - h \cdot f \cdot a - i \cdot d \cdot b}$
    \begin{tikzpicture}[baseline = -0.5ex]
        \matrix [matrix of math nodes,left delimiter=(,right delimiter=)] (m)
        {
            a & b & c & a & b \\
            d & e & f & d & e \\
            g & h & i & g & h \\	
        };
        \draw[] (m-3-3.south east) -- (m-1-3.north east);
        \draw[draw = orange, thick, opacity = 0.5] (m-1-1.north west) -- (m-3-3.south east);
        \draw[draw = orange, thick, opacity = 0.5] (m-1-2.north west) -- (m-3-4.south east);
        \draw[draw = orange, thick, opacity = 0.5] (m-1-3.north west) -- (m-3-5.south east);
        \draw[draw = blue, thick, opacity = 0.5] (m-3-1.south west) -- (m-1-3.north east);
        \draw[draw = blue, thick, opacity = 0.5] (m-3-2.south west) -- (m-1-4.north east);
        \draw[draw = blue, thick, opacity = 0.5] (m-3-3.south west) -- (m-1-5.north east);
    \end{tikzpicture}\\
    ${A}^{-1} = \frac{1}{\det A} \cdot \begin{pmatrix}
        +\det \begin{pmatrix}
            e & f \\
            h & i
        \end{pmatrix} & -\det \begin{pmatrix}
            b & c\\
            h & i
        \end{pmatrix} & +\det \begin{pmatrix}
            b & c \\
            e & f
        \end{pmatrix} \\
        -\det \begin{pmatrix}
            d & f\\
            g & i
        \end{pmatrix} & + \det \begin{pmatrix}
            a & c\\
            g & i
        \end{pmatrix} & - \det \begin{pmatrix}
            a & c\\
            d & f
        \end{pmatrix} \\
        + \det
        \begin{pmatrix}
           d & e\\
           g & h 
        \end{pmatrix} & -\det \begin{pmatrix}
            a & b\\
            g & h
        \end{pmatrix} & + \det \begin{pmatrix}
            a & b \\
            d & e
        \end{pmatrix}
    \end{pmatrix}$
\end{center}
\end{mdframed}
\vspace{-10pt}
\begin{align*}
    \binom{n}{k} := \frac{n!}{k! \cdot (n-k)!}, \qquad
    \binom{n+1}{k} = \binom{n}{k} + \binom{n}{k-1}
\end{align*}
\vspace{-10pt}
\begin{align*}
    (a + b)^n = \summe{i = 0}{n} \binom{n}{i} a^i \cdot b^{(n-i)}
\end{align*}
\vspace{-10pt}
\begin{align*}
    \summe{i = 1}{n} i = \frac{n(n+1)}{2}, \qquad \summe{i = 1}{n} i^2 = \frac{n(n+1)(2n+1)}{6}, \qquad \summe{i = 1}{n} i^3 = \left(\summe{i = 1}{n} i\right)^2 = \frac{n^2(n+2)^2)}{4}
\end{align*}
\vspace{-10pt}
\begin{align*}
    \product{i = 1}{n-1} \left(1 + \frac{1}{i}\right)^i = \frac{n^n}{n!}
\end{align*}
\vspace{-10pt}
\begin{align*}
    \frac{x^n - y^n}{x - y} = x^{n-1} + x^{n-2}y + \ldots + xy^{n-2} + y^{n-1}
\end{align*}
\vspace{-10pt}
\mdfsetup{backgroundcolor=blue!08}
\begin{mdframed}
    \vspace{-10pt}
\begin{align*}
    A \in GL(m,K), B \in M(m\times n,K), C \in M(n\times m,K), D \in GL(n,K)\\
    \begin{pmatrix}
        A & B \\
        C & D
    \end{pmatrix}
    = \begin{pmatrix}
        A & 0\\
        C & \mathds{1}_n
    \end{pmatrix}
    \begin{pmatrix}
        \mathds{1}_m & A^{-1}B\\
        0 & D - CA^{-1}B
    \end{pmatrix} = \begin{pmatrix}
        \mathds{1}_m & B \\
        0 & D
    \end{pmatrix} 
    \begin{pmatrix}
        A - BD^{-1}C & 0\\
        D^{-1}C & \mathds{1}_n
    \end{pmatrix}\\
    \implies 
    \det \begin{pmatrix}
        A & B\\
        C & D
    \end{pmatrix}
    = \det (A) \cdot \det (D - CA^{-1}B) = \det (D) \cdot \det(A - BD^{-1}C) 
\end{align*}
\end{mdframed}
\textbf{Vandermonde Determinante}
\begin{align*}
    V(x_1, \ldots, x_n) = \begin{pmatrix}
        1 & x_1 & x_1^2 & \ldots & x_1^{n-1}\\
        1 & x_2 & x_2^2 & \ldots & x_2^{n-1}\\
        \vdots & & & \ddots &\\
        1 & x_n & x_n^2 & \ldots & x_n^{n-1}
    \end{pmatrix}\\
    \det V(x_1, \ldots, x_n) = \underset{1 \leq i < j \leq n}{\prod} (x_j - x_i)
\end{align*}
