\begin{empheq}[box=\bluebase]{align*}
    \begin{array}{c}
        A \in GL(m,K), b \in M(m\times n,K), C \in M(n\times m,K), D \in GL(n,K)\\
        \begin{pmatrix}
            A & B\\
            C & D
        \end{pmatrix}
            = \begin{pmatrix}
            A & 0\\
            C & E_n
        \end{pmatrix}
        \begin{pmatrix}
            E_m & A^{-1}B\\
            0 & D - CA^{-1}B
        \end{pmatrix}
        = \begin{pmatrix}
            E_m & B\\
            0 & D
        \end{pmatrix}
        \begin{pmatrix}
            A - BD^{-1}C & 0\\
            D^{-1}C & E_n
        \end{pmatrix}\\
        \implies \det \begin{pmatrix}
            A & B\\
            C & D
        \end{pmatrix} = \det(A) \cdot \det(D - CA^{-1}B) = \det(D) \cdot \det(A - BD^{-1}C)
    \end{array}
\end{empheq}


Die \textbf{Vandermonde Matrix} ist gegeben durch 

\begin{empheq}[box=\bluebase]{align*}
    V(x_1, \ldots, x_n) = \begin{pmatrix}
        1 & x_1 & x_1^2 & \cdots & x_1^{n-1}\\
        1 & x_2 & x_2^2 & \cdots & x_2^{-1}\\
        \vdots & \ddots & \ddots & \vdots\\
        1 & x_n & x_n^2 & \cdots & x_n^{n-1}
    \end{pmatrix}, \quad \det V(x_1, \ldots,x_n) = \prod_{1 \leq i < j \leq n} (x_j - x_i)
\end{empheq}

\begin{empheq}[box=\bluebase]{align*}
    \sum_{i = 1}^{n} i^2 = \frac{n(n+1)(2n+1)}{6}, \quad \sum_{i = 1}^{n}i^3 = \left(\sum_{i = 1}^{n}i\right)^2 = \frac{n^2(n+2)^2}{4}, \quad \prod_{i=1}^{n-1}(1 + \frac{1}{i})^i = \frac{n^n}{n!}
\end{empheq}
