
$$
\Phi_{\Delta t}^{(1)} : \quad
\left\{\begin{array}{ll}
    p^{k + 1} = p^{k}
    \\
  q^{k+ 1} = q^k + \Delta t p^k
\end{array} \right.
$$
$$
\Phi_{\Delta t}^{(2)}: \quad
\left\{\begin{array}{ll}
    p^{k+1} = p^{k } - \Delta t q^{k }
    \\
    q^{k+1} = q^{k }
\end{array} \right.
$$

whose adjoints can be obtained by exchanging the indices $k$,$k+ \frac{1}{2}$ with $k+\frac{1}{2},k+1$, respectively and changing the sign of $\Delta t$.

$$
(\Phi_{\Delta t}^{(1)})^{*} : \quad
\left\{\begin{array}{ll}
    p^{k + 1} = p^{k}
    \\
  q^{k+ 1} = q^k + \Delta t p^{k+ 1}
\end{array} \right.
$$
$$
(\Phi_{\Delta t}^{(2)})^{\ast}: \quad
\left\{\begin{array}{ll}
    p^{k+1} = p^{k } - \Delta t q^{k + 1}
    \\
    q^{k+1} = q^{k }
\end{array} \right.
$$

Since $(\Phi_{\Delta t}^{(2)} \circ \Phi_{\Delta t}^{(1)})^{\ast} = (\Phi_{\Delta t}^{(1)})^{\ast} \circ (\Phi_{\Delta t}^{(2)})^{\ast}$.
