\subsection{The Lebesgue-Stieltjes Measure}


Let $F: \R \to \R$ be non-decreasing and continuous from the left, i.e: 
\begin{align*}
  F(x_0) = \lim_{x \to x_0^{-}}F(x) := \lim_{\underset{x < x_0}{x \to x_0}} F(x) \quad \forall x_0 \in \R
\end{align*}
For $a,b$ we define
\begin{align*}
  \lambda_F[a,b) = \left\{\begin{array}{ll}
      F(b) - F(a) & \text{ if }a < b\\
    0 & \text{ otherwise}
  \end{array} \right.
\end{align*}

Because the collection of bounded half-open sets
$
  \mathcal{K} = \{[a,b)\big\vert a,b \in \R\}
$
does not form an Algebra (see \ref{rem:half-open-ring}), 
we cannot use the Carathéodory-Hahn extension theorem to produce a measure induced by $\lambda_F$.

However, $\mathcal{K}$ constitutes a covering of $\R$ as in Definition \ref{dfn:covering},
so by Theorem \ref{thm:cover-to-measure}, the function $\lambda_F$ induces a measure
\begin{align*}
  \Lambda_F(A) := \inf \left\{
    \sum_{k=1}^{\infty} \lambda_F[a_k,b_k), \quad A \subseteq \bigcup_{k=1}^{\infty}[a_k,b_k)
  \right\}
\end{align*}
called the \textbf{Lebesgue-Stieltjes Measure} generated by $F$.


To find out if $\Lambda_F$ is nice, we will find the following definition useful.
\begin{dfn}[]
A measure $\mu$ on $\R^{n}$ is called \textbf{metric,} if the measure is additive on separated sets, 
i.e. for all $A,B \subseteq \R^{n}$ with
\begin{align*}
  \text{dist}(A,B) := \inf \{\abs{a-b}, a \in A, b \in B\} > 0
\end{align*}
it holds
\begin{align*}
  \mu(A \cup B) = \mu(A) + \mu(B)
\end{align*}
\end{dfn}
By subadditivity, the inequality ``$\geq$'' is sufficient.


\begin{thm}[Carathéodory criterion for Borel measures]
  \label{thm:metric-is-borel}
  A metric measure $\mu$ on $\R^{n}$ is Borel.
\end{thm}
\begin{proof}
  Let $\mu$ be a metric measure on $\R^{n}$.
  Because the $\mu$-measurable subsets (\ref{thm:measurable-is-sigma-algebra}) form a $\sigma$-Algebra, it is sufficient to show that closed sets are $\mu$-measurable.


  Let $F \subseteq \R^{n}$ be closed and $B \subseteq \R^{n}$ be some test set.
  If $\mu(B) = \infty$, then the inequality
  \begin{align*}
    \mu(B) \geq \mu(B \cap F) + \mu(B \setminus F)
  \end{align*}
  is trivial, so assume $\mu(B) < \infty$.
  For $k = 1, 2, \ldots$, we define
  \begin{align*}
    F_k := \{x \in \R^{n} \big\vert 0 \leq \text{dist}(x,F) \leq \frac{1}{k}\}
  \end{align*}
  It should be clear that 
  \begin{align*}
    \text{dist}(B \setminus F_k, B \cap F) \geq \frac{1}{k} > 0
  \end{align*}
  so since $\mu$ is metric and monotonous, we have
  \begin{align*}
    \mu(B \cap F) + \mu(B \setminus F_k) = \mu((B \cap F) \cup (B \setminus F_k)) \leq \mu(B) \quad \forall k
  \end{align*}
  If we can show that $\lim_{k \to \infty} \mu(B \cap F_k) = \mu(B \setminus F)$, then we are done.

  To do so, first note that the $(F_k)_{k \in \N}$ form a decreasing sequence $F_{k+1} \subseteq F_k$.
  Moreover, we have $F = \bigcap_{k=1}^{\infty} F_k$, so we can write
  \begin{align*}
    B \setminus F
    =
    B \setminus \bigcap_{l=1}^{\infty}F_l
    = \bigcup_{l=1}^{\infty} (B \setminus F_l)
  \end{align*}
  We can expand the union above in telescoping fashion
  \footnote{
    For example, for any sequence $(A_l)_{l \in \N}$ we can write $\bigcup_{l=1}^{\infty} A_l = A_1 \cup \bigcup_{l=1}^{\infty}A_{l+1} \setminus A_l$.
  }
  and use the fact that the $(B \setminus F_l)_{l \in \N}$ form an increasing sequence to get
  \begin{align*}
    \bigcup_{l=1}^{\infty}(B \setminus F_l) 
    &=
    (B \setminus F_1) \cup \bigcup_{l=1}^{\infty}(B \setminus F_{l+1}) \setminus (B \setminus F_l)\\
    &=
    (B \setminus F_k) \cup \bigcup_{l=k}^{\infty} (F_l \setminus F_{l+1}) \cap B
  \end{align*}
  Setting
  \begin{align*}
    R_l := (F_l \setminus F_{l+1}) \cap B = \{x \in B \big\vert \frac{1}{l+1} < d(x,F) \leq \frac{1}{l}\}
  \end{align*}
  we see that the $(R_l)_{l \in \N}$ are pairwise disjoint, so we have
  \begin{align*}
    B \setminus F = (B \setminus F_k) \cup \bigsqcup_{l=k}^{\infty} R_l
  \end{align*}
  Therefore, for all $k \in \N$ it holds
  \begin{align*}
    \mu(B \setminus F_k) \leq \mu(B \setminus F) \leq \mu(B \setminus F_k) + \sum_{l=k}^{\infty} \mu(R_l)
  \end{align*}
  Now we only need to show that
  \begin{align*}
    \lim_{k \to \infty} \sum_{l=k}^{\infty} \mu(R_l) = 0
  \end{align*}

  Observe that $R_i$ only ``touches'' its neighbors $R_{i-1},R_{i+1}$, in other words
  \begin{align*}
    \text{dist}(R_i,R_j) > 0, \quad \text{ if } \abs{i-j} \geq 2
  \end{align*}
  decomposing the sum $\sum_{l=1}^{\infty} \mu(R_l)$ into the even and odd numbers,
  we can use the fact that $\mu$ is metric to get
  \begin{align*}
    \sum_{l=1}^{2m + 1} \mu(R_l) = 
    \left(\sum_{k=1}^{m} \mu(R_{2k})\right)
      +
    \left(
      \sum_{k=1}^{m} \mu(R_{2k})
    \right)
    = \mu \left(
        \bigcup_{k=1}^{m} R_{2k}
      \right)
      +
    \mu \left(
      \bigcup_{k=1}^{m} R_{2k}
    \right)
    \leq 2 \mu(B) < \infty
  \end{align*}
  so even in the limit $m \to \infty$, the series converges.
  But in the inequality we showed earlier
  \begin{align*}
    \mu(B \setminus F_k) \leq \mu(B \setminus F) \leq \mu(B \setminus F_k) + \sum_{l=k}^{\infty} \mu(R_l)
  \end{align*}
  we were allowed to omit any number of (non-negative) starting terms $\mu(R_l)$ for $l < k$, so in the limit we get $\lim_{k \to \infty} \mu(B \setminus F_k) = \mu(B \setminus F)$, and the result follows.
\end{proof}


\begin{thm}[] \label{thm:stieltjes-is-borel-regular}
  The Lebesgue-Stieltjes measure $\Lambda_F$ is Borel regular.
\end{thm}
\begin{proof}
  \begin{enumerate}[{(}i{)}]
    \item $\bm{\Lambda_F}$ \textbf{is Borel.}
  We show that it is metric and use the previous theorem, so let $A,B \subseteq \R$ with $\delta := \text{dist}(A,B) > 0$.
  We now show that for all $\epsilon > 0$ we have
  \begin{align*}
    \Lambda_F(A) + \Lambda_F(B) \leq \Lambda_F(A \cup B) + \epsilon
  \end{align*}

  Per definition of the Lebesgue-Stieltjes measure, we can find a collection of half-open intervals with
  \begin{align*}
    A \cup B \subseteq \bigcup_{k=1}^{\infty} [a_k,b_k) \quad \text{and} \quad \sum_{k=1}^{\infty} < \Lambda_F(A \cup B) + \epsilon
  \end{align*}
  Because we can always subdivide any interval $[a_k,b_k)$ further, we may also assume that $\abs{b_k - a_k} < \delta$ for all $k$.

  Because $A$ and $B$ are separated, for each interval $[a_k,b_k)$ either
  \begin{align*}
    A \cap  [a_k,b_k) = \emptyset \quad \text{or} \quad 
    B \cap  [a_k,b_k) = \emptyset 
  \end{align*}
  , so the covering of $A \cup B$ gives us a covering $\mathcal{A}$ of $A$ and a covering $\mathcal{B}$ of $B$.
  Therefore
  \begin{align*}
    \Lambda_F(A) + \Lambda_F(B) 
    &\leq 
    \sum_{[a_k,b_k) \in \mathcal{A}} \Lambda_F([a_k,b_k))
    +
    \sum_{[a_k,b_k) \in \mathcal{B}} \Lambda_F([a_k,b_k))\\
    &= \sum_{k\in \N} \lambda_F([a_k,b_k) \leq \Lambda_F(A \cup B) + \epsilon
  \end{align*}
  This shows that $\Lambda_F$ is metric and thus Borel.

  \item $\bm{\Lambda_F}$ \textbf{is Borel regular.}

  To show that $\Lambda_F$ is Borel regular, let $A \subseteq \R$.
  Of course we can assume $\Lambda_F(A) < \infty$.
  Then for any $n \in \N$ we can find coverings 
  \begin{align*}
    A \subseteq \bigcup_{k=1}^{\infty} \left[a_k^{(n)},b_k^{(n)}\right) =: B_n 
    \quad \text{with} \quad 
    \sum_{k=1}^{\infty} \lambda_F\left(\left[a_k^{(n)},b_k^{(n)}\right)\right) \leq \Lambda_F(A) + \frac{1}{n}
  \end{align*}
  If we set $B := \bigcap_{n=1}^{\infty}B$, then $B$ is Borel and $A \subseteq B \subseteq B_n$ and 
  \begin{align*}
    \Lambda_F(A) \leq \Lambda_F(B) \leq \Lambda_F(B_n) 
    \leq 
    \sum_{k=1}^{\infty}\lambda_F\left(\left[a_k^{(n)},b_k^{(n)}\right)\right) \leq \Lambda_F(A) + \frac{1}{n}
  \end{align*}
  in the limit $n \to \infty$, we get $\Lambda_F(A) = \Lambda_F(B)$, so $\Lambda_F$ is Borel regular.
  \end{enumerate}
\end{proof}


The Carathéodory-Hahn extension had the property that it coincided with the pre-measure on the algebra, on which the pre-measure was defined.
Despite not being such an extension, the Lebesgue-Stieltjes measure has a similar property.

\begin{thm}[]
For $a<b \in \R$ it holds
\begin{align*}
  \Lambda_F \left(
    [a,b)
  \right)
  = \lambda_F\left(
    [a,b)
  \right)
  = F(b) - F(a)
\end{align*}
\end{thm}
\begin{proof}
  Let $a<b \in \R$. By definition of $\Lambda_F$, we already have $\Lambda_F([a,b)) \leq \lambda_F([a,b))$.

  For the other inequality, let $\left(
    [a_k,b_k)
  \right)_{k \in \N}$ be a covering of $[a,b)$.

  Since $F$ is left-continuous, for every $\epsilon> 0$ there exist $\delta, \delta_k > 0$ such that
  \begin{align*}
    F(b) - F(b - \delta) \leq \epsilon, \quad \text{and} \quad F(a_k) - F(a_k - \delta_k) \leq 2^{-k} \epsilon \quad \forall k \in \N
  \end{align*}
  Because $[a, b - \delta]$ is compact and is covered by $\bigcup_{k=0}^{\infty}(a_k - \delta_k,b_k)$, there exists a finite subcovering
  \begin{align*}
    [a, b- \delta] \subseteq \bigcup_{k=0}^{m}(a_k - \delta_k, b_k)
  \end{align*}
  By removing any redundant intervals, we can decrease the sum $\sum_{k=0}^{m} \lambda_F(a_k - \delta_k,b_k)$, so we can assume WLOG that they are ordered in such a way that 
  \begin{align*}
    a_k - \delta_k < b_{k-1} \quad \text{for all} \quad k = 1, \ldots, m
  \end{align*}
  
  Since $F$ is increasing and $a_0 - \delta_0 < a < b < b_m$, we have
  \begin{align*}
    %\lambda_F([a, b - \delta)) 
    %&=
    F(b- \delta) - F(a) 
    &\leq F(b_m) - F(a_0 - \delta_0)\\
    &\leq F(b_m) 
    - F(a_1 - \delta_1) 
    + F(b_0)
    - F(a_0 - \delta_0)\\
    &\leq \ldots \leq
    \sum_{k=0}^{m}F(b_k) - F(a_k - \delta_k)
  \end{align*}
  so with the initial estimates, we have
  \begin{align*}
    \lambda_F([a,b)) 
    &= F(b) - F(a)
    =
    F(b) - F(b - \delta) + F(b - \delta) - F(a)\\
    &\leq \epsilon + \sum_{k=0}^{m} F(b_k) - F(a_k - \delta_k)\\
    &= \epsilon + \sum_{k=0}^{m} F(b_k) - F(a_k) + \sum_{k=0}^{m} F(a_k) - F(a_k - \delta_k)\\
    &\leq \epsilon + \sum_{k=0}^{\infty}F(b_k) - F(a_k) + \sum_{k=0}^{\infty} 2^{-k} \epsilon\\
    &= \sum_{k=0}^{\infty} \lambda_F([a_k,b_k)) + 3 \epsilon
  \end{align*}
  Since this is true for all coverings $([a_k,b_k))_{k \in \N}$, we get in the limit $\epsilon \to 0$
  \begin{align*}
    \lambda_F([a,b)) \leq \Lambda_F([a,b))
  \end{align*}
\end{proof}


\begin{ex}[]
\phantom{a}
\begin{itemize}
  \item The Lebesgue measure is the special case when $F(x) = x$, so $\Lambda_{\id_{\R}} = \Leb^{1}$
  \item The Dirac measure $\delta_0$ from Example \ref{ex:dirac-counting-indiscrete} is the Lebesgue-Stieltjes measure $\Lambda_{\Theta}$ for the Heaviside step function
    \begin{align*}
      \Theta(x) = \left\{\begin{array}{ll}
        1 & x > 0\\
        0 & x \leq 0
      \end{array} \right.
    \end{align*}
\end{itemize}
\end{ex}
