
\section{Appendix}

\subsection{Distributions}

\subsubsection*{Poisson Distribution with parameter $\lambda$}

\begin{align*}
  \Omega = \{0,1,2,\ldots\}, \quad \IP[X=n] = e^{-\lambda} \frac{\lambda^{n}}{n!}
\end{align*}

\begin{align*}
  X \sim \text{Poi}(\lambda), Y \sim \text{Poi}(\mu) \text{ independent} \implies X +Y \sim \text{Poi}(\lambda + \mu)
\end{align*}
\begin{proof}
  For $S = X + Y$
  \begin{align*}
    \IP[S = s] 
    &= \sum_{k=0}^{s} \IP[X = k, Y = s-k]\\
    &= \sum_{k=0}^{s} \IP[X = k] \cdot \IP[Y = s-k]\\
    &= \sum_{k=0}^{s} e^{- \lambda} \frac{\lambda^{s}}{s!} e^{- \mu} \frac{\mu^{k-s}}{(s-k)!}\\
    &= \frac{e^{-\lambda + \mu}}{s!}\sum_{k=0}^{s} \binom{s}{k} \lambda^{k} \mu^{s-k}\\
    &= \frac{e^{-\lambda + \mu}}{s!} (\lambda + \mu)^{s}
  \end{align*}
\end{proof}




\subsection{Theorems}

\subsubsection*{Borel Cantelli}

Let $A_1,A_2, \ldots \in \mathcal{A}$. Set
\begin{align*}
  A_{\infty} := \limsup_{n = \infty} = \bigcap_{n=1}^{\infty} \bigcup_{k=1}^{n} A_k
\end{align*}
then
\begin{enumerate}
  \item $\sum_{k=1}^{\infty} \IP[A_k] < \infty \implies \IP[A_{\infty}] = 0$
  \item If the $(A_k)_{k \in \N}$ are independent, then $\sum_{k=1}^{\infty} \IP[A_k] = \infty \implies \IP[A_{\infty}] = 1$.
\end{enumerate}



\subsection{Gaussian/Normal Distribution with parameters $\mu,\sigma^{2}$}

For $\mu,\sigma \in \R,\sigma > 0$ the density for $\mathcal{N}(\mu,\sigma^{2}$ is given by
\begin{align*}
  f(x) = \frac{1}{\sigma \sqrt{2 \pi}} \exp\left(
    - \frac{(x - \mu)^{2}}{2 \sigma^{2}}
  \right)
\end{align*}
$\mu$ is called the \textbf{mean} and for 
$X \sim \mathcal{N}(\mu,\sigma^{2})$ is the expectation value $\E[X] = \mu$.
$\sigma$ is called the \textbf{standard deviation} and $\sigma^{2} =: \variance(X)$ the \textbf{variance}

\begin{lem}[]
  For $X \sim \mathcal{N}(\mu_X,\sigma_X^{2})$ and $Y \sim \mathcal{N}(\mu_Y,\sigma_Y^2)$ independent, their sum is also normal distributed with parameters
  \begin{align*}
    Z = X + Y \sim \mathcal{N}(\mu_X + \mu_Y, \sigma_X^{2} + \sigma_Y^{2})
  \end{align*}
\end{lem}
\begin{proof}
  Since $\IP[Z = z] = \IP[X = x] \cdot \IP[Y = z-x]$, the density of $Z$ is the convolution of the densities of $X$ and $Y$.

\end{proof}


